Test/VerifyThis2015/Problem3.dfy
@@ -1,4 +1,4 @@
-// RUN: %dafny /compile:3 /print:"%t.print" /dprint:"%t.dprint" "%s" > "%t"
+// RUN: %dafny /compile:3 /print:"%t.print" /dprint:"%t.dprint" /vcsMaxKeepGoingSplits:5 "%s" > "%t"
 // RUN: %diff "%s.expect" "%t"
 
 // Rustan Leino
